src/cbor/raw/pulse/everparse/CBOR.Pulse.Raw.Serialized.Base.fst
@@ -25,7 +25,7 @@ fn cbor_read
   let pc = get_header_and_contents input ph;
   let h = !ph;
   let typ = ((get_header_initial_byte h).major_type);
-  if (typ = cbor_major_type_uint64) {
+  if (typ = cbor_major_type_uint64 || typ = cbor_major_type_neg_int64) {
     elim_trade _ _;
     let i = get_int64_value v h;
     cbor_match_int_intro_trade (pts_to_serialized serialize_raw_data_item input #pm v) typ i
@@ -38,8 +38,20 @@ fn cbor_read
     Trade.trans _ _ (pts_to_serialized serialize_raw_data_item input #pm v);
     res
   }
-  else {
+  else if (typ = cbor_major_type_tagged) {
     admit ()
+  }
+  else if (typ = cbor_major_type_array) {
+    admit ()
+  }
+  else if (typ = cbor_major_type_map) {
+    admit ()
+  }
+  else {
+    assert (pure (typ == cbor_major_type_simple_value));
+    elim_trade _ _;
+    let i = get_simple_value v h;
+    cbor_match_simple_intro_trade (pts_to_serialized serialize_raw_data_item input #pm v) i
   }
 }
 ```
